\section{Appendix}

\subsection{Mean model of the position update component}
\label{app:mean_pso}

By applying mean to \eqref{eq:pso_up_linalg_simp}, we can have the mean of the position update component as
\begin{equation}
\label{eq:pso_up_linalg_simp:mean}
E( X(k+1) ) = A(k) E( X(k) ) + B(k) E( U(k) )
\end{equation}
with
$ A(k) = \begin{bmatrix}
\chi & - \chi \phi^{G}/2 - \chi \phi^{P}/2
\\ 
\chi & 1 - \chi \phi^{G}/2 - \chi \phi^{P}/2
\end{bmatrix} $
and
$ B(k) = \begin{bmatrix}
\chi \phi^{G}/2 & \chi \phi^{P}/2
\\ 
\chi \phi^{G}/2 & \chi \phi^{P}/2
\end{bmatrix} $.

$ E( X(k) ) = [ E( v(k) ), E( x(k) - x^{R} ) ]^{T} $ and $ E( U(k) ) = [ E( x^{G}(k) - x^{R} ) , E( x^{P}(k) - x^{R} ) ]^{T} $.

By taking $ x^{R} = x^{*} $, we can have \eqref{eq:mean:opt_bound}.
